@prefix rdf: <http://www.w3.org/1999/02/22-rdf-syntax-ns#> .
@prefix rdfs: <http://www.w3.org/2000/01/rdf-schema#> .
@prefix xsd: <http://www.w3.org/2001/XMLSchema#> .
@prefix owl: <http://www.w3.org/2002/07/owl#> .
@prefix xdd: <http://terminusdb.com/schema/xdd#> .
@prefix system: <http://terminusdb.com/schema/system#> .
@prefix layer: <http://terminusdb.com/schema/layer#> .

<http://terminusdb.com/schema/system>
  a owl:Ontology ;
  rdfs:label "Terminus DB Management Schema"@en ;
  rdfs:comment "Schema describing all of the structure of the documents (capabilities, roles, resources, users, databases) in the capability database used by Terminus DB to manage the internal state of the server and the databases it manages"@en ;
  system:rights "Copyright Data Chemist Ltd. 2017-2019"@en ;
  system:author "Gavin Mendel-Gleason"@en, "Kevin C. Feeney"@en ;
  system:license <https://creativecommons.org/licenses/by-sa/2.0/>, <https://www.gnu.org/licenses/gpl-3.0.en.html> .

system:Document
  a owl:Class ;
  system:tag system:abstract ;
  rdfs:label "Document Class"@en ;
  rdfs:comment "A class used to designate the primary data objects managed by the system - relationships and entities"@en .

system:Agent
  rdfs:label "Agent"@en ;
  rdfs:comment "An agent is an abstraction of a thing that can have a capability"@en ;
  a owl:Class ;
  system:tag system:abstract ;
  rdfs:subClassOf system:Document .

system:rights
  a owl:DatatypeProperty ;
  rdfs:range xsd:string ;
  rdfs:domain owl:Ontology ;
  rdfs:label "Rights"@en ;
  rdfs:comment "The statement of rights of the owner"@en .

system:author
  a owl:DatatypeProperty ;
  rdfs:domain owl:Ontology ;
  rdfs:range xsd:string ;
  rdfs:label "Author"@en ;
  rdfs:comment "The authors who developed the ontology"@en .

system:license
  a owl:ObjectProperty ;
  rdfs:domain owl:Ontology ;
  rdfs:range owl:Thing ;
  rdfs:label "License"@en ;
  rdfs:comment "The license governing the use of the resource"@en .

system:role
  rdfs:label "Has Role"@en ;
  rdfs:comment "A property that links an agent has a role"@en ;
  a owl:ObjectProperty ;
  rdfs:domain system:Agent ;
  rdfs:range system:Role .

system:Role
  rdfs:label "Role"@en ;
  rdfs:comment "A role is a collection of capabilities that can be allocated to any user"@en ;
  a owl:Class ;
  rdfs:subClassOf system:Document .

system:User
  rdfs:label "User"@en ;
  rdfs:comment "A user of the database"@en ;
  a owl:Class ;
  rdfs:subClassOf system:Agent .

system:Organization
  rdfs:label "Organization"@en ;
  rdfs:comment "An organization or team"@en ;
  a owl:Class ;
  rdfs:subClassOf system:Resource .

system:organization_name
  a owl:DatatypeProperty ;
  rdfs:subPropertyOf system:resource_name ;
  rdfs:label "organization name"@en ;
  rdfs:comment "The name of an organization"@en ;
  rdfs:domain system:Organization ;
  rdfs:range xsd:string .

system:organization_child
  a owl:ObjectProperty ;
  rdfs:subPropertyOf system:resource_includes ;
  rdfs:domain system:Organization ;
  rdfs:range system:Organization .

system:organization_database
  a owl:ObjectProperty ;
  rdfs:subPropertyOf system:resource_includes ;
  rdfs:domain system:Organization ;
  rdfs:range system:Database .

system:user_identifier
  rdfs:label "User Identifier"@en ;
  rdfs:comment "Default identifier used for a user"@en ;
  a owl:DatatypeProperty ;
  rdfs:domain system:User ;
  rdfs:range xsd:string .

system:CapabilityScopeRestriction
  a owl:Restriction ;
  rdfs:label "Capability Scope Restriction"@en ;
  rdfs:comment "Exactly one capability scope per capability"@en ;
  rdfs:onProperty system:capability_scope ;
  owl:cardinality "1"^^xsd:nonNegativeInteger .

system:Capability
  a owl:Class ;
  rdfs:subClassOf system:Document, system:CapabilityScopeRestriction ;
  rdfs:label "Capability"@en ;
  rdfs:comment "A capability confers access to a database or server action"@en .

system:capability
  a owl:ObjectProperty ;
  rdfs:label "capability"@en ;
  rdfs:comment "associates a role with its capabilities"@en ;
  rdfs:domain system:Role ;
  rdfs:range system:Capability .

system:capability_scope
  a owl:ObjectProperty ;
  rdfs:label "Capability Scope"@en ;
  rdfs:comment "The scope of a capability - the resource that the capability applies to"@en ;
  rdfs:domain system:Capability ;
  rdfs:range system:Resource .

system:direct_capability_scope
  a owl:ObjectProperty ;
  rdfs:subPropertOf system:capability_scope ;
  rdfs:label "Direct Capability Scope"@en ;
  rdfs:comment "The direct resource controlled by a capability - not a transitive property"@en ;
  rdfs:domain system:Capability ;
  rdfs:range system:Resource .

system:resource_includes
  rdfs:label "Resource Inclusion"@en ;
  rdfs:comment "Resource A includes Resource B if A resource_includes B i.e. A Server might include a Database within its scope"@en ;
  a owl:ObjectProperty ;
  rdfs:domain system:Resource ;
  rdfs:range system:Resource .

system:action
  rdfs:label "Action"@en ;
  rdfs:comment "Refers to a specific API access call"@en ;
  a owl:ObjectProperty ;
  rdfs:domain system:Capability ;
  rdfs:range system:DBAction .

system:DBAction
  rdfs:label "DB Action"@en ;
  a owl:Class ;
  owl:oneOf (
    system:create_database
    system:delete_database
    system:class_frame
    system:clone
    system:fetch
    system:push
    system:branch
    system:rebase
    system:instance_read_access
    system:instance_write_access
    system:schema_read_access
    system:schema_write_access
    system:inference_read_access
    system:inference_write_access
    system:meta_read_access
    system:meta_write_access
    system:commit_read_access
    system:commit_write_access
    system:manage_capabilities
    ).

system:delete_database
  rdfs:label "Delete Database"@en ;
  rdfs:comment "An action that deletes an entire database"@en ;
  a system:DBAction.

system:schema_write_access
  rdfs:label "Update Schema"@en ;
  rdfs:comment "An action that updates the DB schema"@en ;
  a system:DBAction.

system:schema_read_access
  rdfs:label "Get Schema"@en ;
  rdfs:comment "An action that fetches the DB Schema"@en ;
  a system:DBAction.

system:inference_write_access
  rdfs:label "Update Inference"@en ;
  rdfs:comment "An action that updates the DB inference"@en ;
  a system:DBAction.

system:inference_read_access
  rdfs:label "Get Inference"@en ;
  rdfs:comment "An action that fetches the DB Inference"@en ;
  a system:DBAction.

system:class_frame
  rdfs:label "Class Frame"@en ;
  rdfs:comment "An action that fetches a Frame JSON for the appropriate Class"@en ;
  a system:DBAction.

system:create_database
  rdfs:label "Create Database"@en ;
  rdfs:comment "An action which creates a new database"@en ;
  a system:DBAction.

system:clone
  rdfs:label "Clone"@en ;
  rdfs:comment "An action which represents cloning a database"@en ;
  a system:DBAction .

system:fetch
  rdfs:label "Fetch"@en ;
  rdfs:comment "An action which represents fetching a database from a remote origin"@en ;
  a system:DBAction .

system:push
  rdfs:label "Push"@en ;
  rdfs:comment "An action which represents pushing a database to a remote origin"@en ;
  a system:DBAction .

system:branch
  rdfs:label "Branch"@en ;
  rdfs:comment "An action which represents creating a new branch of a database"@en ;
  a system:DBAction .

system:rebase
  rdfs:label "Rebase"@en ;
  rdfs:comment "An action which represents Rebasing a database branch"@en ;
  a system:DBAction .

system:instance_read_access
  rdfs:label "Instance Read Access"@en ;
  rdfs:comment "An action which allows all read-only instance data accesses to the database"@en ;
  a system:DBAction .

system:instance_write_access
  rdfs:label "Instance Write Access"@en ;
  rdfs:comment "An action which allows all write instance data accesses to the database"@en ;
  a system:DBAction .

system:schema_read_access
  rdfs:label "Schema Read Access"@en ;
  rdfs:comment "An action which allows all read-only schema data accesses to the database"@en ;
  a system:DBAction .

system:schema_write_access
  rdfs:label "Schema Write Access"@en ;
  rdfs:comment "An action which allows all write schema data accesses to the database"@en ;
  a system:DBAction .

system:inference_read_access
  rdfs:label "Inference Read Access"@en ;
  rdfs:comment "An action which allows all read-only inference data accesses to the database"@en ;
  a system:DBAction .

system:inference_write_access
  rdfs:label "Inference Write Access"@en ;
  rdfs:comment "An action which allows all write inference data accesses to the database"@en ;
  a system:DBAction .

system:meta_read_access
  rdfs:label "Meta Read Access"@en ;
  rdfs:comment "An action which allows all read-only meta data accesses to the database"@en ;
  a system:DBAction .

system:meta_write_access
  rdfs:label "Meta Write Access"@en ;
  rdfs:comment "An action which allows meta data write accesses to the database"@en ;
  a system:DBAction .

system:commit_read_access
  rdfs:label "Commit Read Access"@en ;
  rdfs:comment "An action which allows all read-only commit data accesses to the database"@en ;
  a system:DBAction .

system:commit_write_access
  rdfs:label "Commit Write Access"@en ;
  rdfs:comment "An action which allows commit data write accesses to the database"@en ;
  a system:DBAction .

system:manage_capabilities
  rdfs:label "Management Capabilities"@en ;
  rdfs:comment "An action which allows a user to manage capabilities for a database"@en ;
  a system:DBAction .

system:Resource
  rdfs:label "Resource"@en ;
  rdfs:comment "A resource is a thing that can be accessed and given instructions and for which capabilities can be allocated"@en ;
  a owl:Class ;
  system:tag system:abstract ;
  rdfs:subClassOf system:Document .

system:Database
  rdfs:label "Database"@en ;
  rdfs:comment "A resource representing a database hosted on the server."@en ;
  a owl:Class ;
  rdfs:subClassOf system:Resource .

system:SystemDatabase
  rdfs:label "System Database"@en ;
  rdfs:comment "A resource representing a system core database."@en ;
  a owl:Class ;
  rdfs:subClassOf system:Resource .

system:resource_name
  rdfs:label "Resource Name"@en ;
  rdfs:comment "The resource name which is used as an internal local reference."@en ;
  a owl:DatatypeProperty ;
  rdfs:range xsd:string ;
  rdfs:domain system:Resource .

system:finalized
  a system:DatabaseState ;
  rdfs:label "Finalized"@en ;
  rdfs:comment "The database has been fully constructed"@en .

system:deleting
  a system:DatabaseState ;
  rdfs:label "Deleting"@en ;
  rdfs:comment "TerminusDB is in the process of deleting your database"@en .

system:DatabaseState
  rdfs:label "Database State"@en ;
  rdfs:comment "Class for keeping information about the state of a database." ;
  a owl:Class ;
  owl:oneOf ( system:finalized system:deleting ) .

system:database_state
  rdfs:label "State"@en ;
  rdfs:comment "The databases current state"@en ;
  a owl:ObjectProperty ;
  rdfs:range system:DatabaseState ;
  rdfs:domain system:Database .

system:server
  a system:Server ;
  rdfs:label "server"@en .

system:Server
  rdfs:label "Server"@en ;
  rdfs:comment "A Resource Object Representing the Database Server itself"@en ;
  a owl:Class ;
  owl:oneOf (system:server) ;
  rdfs:subClassOf system:Resource .

system:agent_name
  a owl:DatatypeProperty ;
  rdfs:label "Agent name"@en ;
  rdfs:comment "An name for API authentication"@en ;
  rdfs:domain system:Agent ;
  rdfs:range xsd:string .

system:user_key_hash
  a owl:DatatypeProperty ;
  rdfs:label "User Key"@en ;
  rdfs:comment "A user key for API authentication"@en ;
  rdfs:domain system:User ;
  rdfs:range xsd:string .
